rubin-formal/lakefile.lean
@@ -3,4 +3,10 @@ open Lake DSL
 
 package «rubin-formal» where
 
+require std from git
+  "https://github.com/leanprover/std4" @ "v4.6.0"
+
 lean_lib RubinFormal where
+
+lean_exe rubin_conformance where
+  root := `RubinFormal.Conformance.Main
